Rewrote CQ_Operators (without registers)

isabelle-thys/CQ_Operators.thy
@@ -42,151 +42,58 @@ proof (rule CollectI, erule CollectE, rename_tac Q E)
 qed
 
 definition classical_on :: \<open>('c,'a) qregister \<Rightarrow> ('a ell2, 'a ell2) trace_class \<Rightarrow> bool\<close> where
-  \<open>classical_on C \<rho> \<longleftrightarrow> \<rho> = kraus_family_map (apply_qregister_kraus_map C (complete_measurement (range ket))) \<rho>\<close>
+  \<open>classical_on C \<rho> \<longleftrightarrow> kraus_family_map (apply_qregister_kraus_map C (complete_measurement (range ket))) \<rho> = \<rho>\<close>
 
-lift_definition cq_operator_at :: \<open>('c,'a) qregister \<Rightarrow> ('q,'a) qregister \<Rightarrow> ('a ell2, 'a ell2) trace_class \<Rightarrow> 'c \<Rightarrow> ('q ell2, 'q ell2) trace_class\<close> is
-  \<open>\<lambda>C Q \<rho> c. sandwich (tensor_ell2_left (ket c)*) (apply_qregister (qregister_inv (qregister_pair C Q)) \<rho>)\<close>
-proof (rule CollectI, erule CollectE, rename_tac C Q \<rho> c)
-  fix C :: \<open>('c, 'a) qregister\<close> and Q :: \<open>('q, 'a) qregister\<close> and \<rho> :: \<open> 'a ell2 \<Rightarrow>\<^sub>C\<^sub>L 'a ell2\<close> and c :: 'c
-  assume [iff]: \<open>trace_class \<rho>\<close>
-  show \<open>trace_class (sandwich (tensor_ell2_left (ket c)*) *\<^sub>V apply_qregister (qregister_inv (qregister_pair C Q)) \<rho>)\<close>
-  proof -
-    wlog \<open>iso_qregister (qregister_pair C Q)\<close>
-      using negation
-      by (simp add: qregister_inv_non_iso_qregister)
-    then have \<open>qregister_co_dim (qregister_inv (qregister_pair C Q)) = 1\<close>
-      by (simp add: iso_qregister_co_dim iso_qregister_inv_iso)
-    then have \<open>trace_class (apply_qregister (qregister_inv (qregister_pair C Q)) \<rho>)\<close>
-      by (auto intro!: apply_qregister_trace_class iso_qregister_inv_iso)
-    then show \<open>trace_class (sandwich (tensor_ell2_left (ket c)*) *\<^sub>V apply_qregister (qregister_inv (qregister_pair C Q)) \<rho>)\<close>
-      by (rule trace_class_sandwich)
-  qed
-qed
+definition classical_fst :: \<open>(('c\<times>'q) ell2, ('c\<times>'q) ell2) trace_class \<Rightarrow> bool\<close> where
+  \<open>classical_fst \<rho> \<longleftrightarrow> kraus_family_map (kraus_family_tensor (complete_measurement (range ket)) kraus_family_id) \<rho> = \<rho>\<close>
 
-lemma cq_operator_at_non_partition:
-  assumes \<open>\<not> iso_qregister (qregister_pair C Q)\<close>
-  shows \<open>cq_operator_at C Q \<rho> c = 0\<close>
-  apply (transfer fixing: C Q)
-  using assms
-  by (simp add: qregister_inv_non_iso_qregister)
+(* lemma \<open>classical_fst \<rho> \<longleftrightarrow> classical_on qFst \<rho>\<close>
+  apply (simp add: classical_on_def classical_fst_def)
+  by x *)
 
+definition cq_operator_at :: \<open>(('c\<times>'q) ell2, ('c\<times>'q) ell2) trace_class \<Rightarrow> 'c \<Rightarrow> ('q ell2, 'q ell2) trace_class\<close> where
+  \<open>cq_operator_at \<rho> c = sandwich_tc (tensor_ell2_left (ket c)*) \<rho>\<close>
 
-definition cq_operator_reconstruct :: \<open>('c,'a) qregister \<Rightarrow> ('q,'a) qregister \<Rightarrow> ('c \<Rightarrow> ('q ell2, 'q ell2) trace_class) \<Rightarrow> ('a ell2, 'a ell2) trace_class\<close> where
-  \<open>cq_operator_reconstruct C Q \<rho> = (\<Sum>\<^sub>\<infinity>c. Abs_trace_class (apply_qregister (qregister_pair C Q) (selfbutter (ket c) \<otimes>\<^sub>o from_trace_class (\<rho> c))))\<close>
+definition cq_operator_reconstruct :: \<open>('c \<Rightarrow> ('q ell2, 'q ell2) trace_class) \<Rightarrow> (('c\<times>'q) ell2, ('c\<times>'q) ell2) trace_class\<close> where
+  \<open>cq_operator_reconstruct \<rho> = (\<Sum>\<^sub>\<infinity>c. tc_tensor (tc_butterfly (ket c) (ket c)) (\<rho> c))\<close>
 
 lemma cq_operator_at_summable:
-  fixes C :: \<open>('c, 'a) qregister\<close> and Q :: \<open>('q, 'a) qregister\<close> and \<rho> :: \<open>('a ell2, 'a ell2) trace_class\<close> and c :: 'c
-  shows \<open>cq_operator_at C Q \<rho> abs_summable_on UNIV\<close>
-proof (transfer fixing: C Q, erule CollectE)
-  fix \<rho> :: \<open>'a ell2 \<Rightarrow>\<^sub>C\<^sub>L 'a ell2\<close>
-  define CQi \<rho>' where \<open>CQi = qregister_inv (qregister_pair C Q)\<close> and \<open>\<rho>' = Abs_trace_class (apply_qregister CQi \<rho>)\<close>
-  assume \<open>trace_class \<rho>\<close>
-  show \<open>(\<lambda>x. trace_norm (sandwich (tensor_ell2_left (ket x)*) *\<^sub>V apply_qregister CQi \<rho>)) summable_on UNIV\<close>
-  proof -
-    wlog \<open>iso_qregister (qregister_pair C Q)\<close>
-      by (simp add: negation qregister_inv_non_iso_qregister CQi_def)
-    then have dim: \<open>qregister_co_dim CQi = 1\<close>
-      by (simp add: CQi_def iso_qregister_co_dim iso_qregister_inv_iso)
-    with \<open>trace_class \<rho>\<close> 
-    have CQi\<rho>: \<open>apply_qregister CQi \<rho> = from_trace_class \<rho>'\<close>
-      by (simp add: \<rho>'_def Abs_trace_class_inverse apply_qregister_trace_class)
-    then have rewrite_norm: \<open>trace_norm (sandwich (tensor_ell2_left (ket x)*) (from_trace_class \<rho>'))
-      = norm (sandwich_tc (tensor_ell2_left (ket x)*) \<rho>')\<close> for x
-      by (simp add: from_trace_class_sandwich_tc norm_trace_class.rep_eq)
-    from partial_trace_abs_summable'[of \<open>sandwich_tc swap_ell2 \<rho>'\<close>]
-    have \<open>(\<lambda>x. sandwich_tc (tensor_ell2_left (ket x)*) \<rho>') abs_summable_on UNIV\<close>
-      by (auto intro!: simp: sandwich_tc_compose[symmetric, unfolded o_def, THEN fun_cong])
-    then show ?thesis
-      by (simp add: CQi\<rho> rewrite_norm)
-  qed
-qed
-
+  fixes \<rho> :: \<open>(('c\<times>'q) ell2, ('c\<times>'q) ell2) trace_class\<close> and c :: 'c
+  shows \<open>cq_operator_at \<rho> abs_summable_on UNIV\<close>
+  using partial_trace_abs_summable'[of \<open>sandwich_tc swap_ell2 \<rho>\<close>]
+  by (simp add: cq_operator_at_def sandwich_tc_compose[symmetric, unfolded o_def, THEN fun_cong])
 
 lemma cq_operator_at_bounded_clinear[bounded_clinear]:
-  \<open>bounded_clinear (\<lambda>\<rho>. cq_operator_at C Q \<rho> c)\<close>
+  \<open>bounded_clinear (\<lambda>\<rho>. cq_operator_at \<rho> c)\<close>
 proof -
-  wlog iso: \<open>iso_qregister (qregister_pair C Q)\<close>
-    using cq_operator_at_non_partition[OF negation]
-    by simp
-  then have dim: \<open>qregister_co_dim (qregister_inv (qregister_pair C Q)) = 1\<close>
-    using iso_qregister_co_dim iso_qregister_inv_iso by blast
-
-  have 1: \<open>cq_operator_at C Q (x + y) c = cq_operator_at C Q x c + cq_operator_at C Q y c\<close> for x y
-    apply (transfer' fixing: C Q c)
-    by (simp add: apply_qregister_plus cblinfun.add_right)
-  have 2: \<open>cq_operator_at C Q (r *\<^sub>C x) c = r *\<^sub>C cq_operator_at C Q x c\<close> for x r
-    apply (transfer' fixing: C Q c)
-    by (simp add: apply_qregister_scaleC cblinfun.scaleC_right)
-  have 3: \<open>norm (cq_operator_at C Q x c) \<le> norm x * 1\<close> for x
-  proof (transfer fixing: C Q c, erule CollectE)
-    fix x :: \<open>'a ell2 \<Rightarrow>\<^sub>C\<^sub>L 'a ell2\<close>
-    assume \<open>trace_class x\<close>
-    then have tc: \<open>trace_class (apply_qregister (qregister_inv (qregister_pair C Q)) x)\<close>
-      by (auto intro!: apply_qregister_trace_class iso_qregister_inv_iso simp: dim)
-    have \<open>trace_norm (sandwich (tensor_ell2_left (ket c)*) *\<^sub>V apply_qregister (qregister_inv (qregister_pair C Q)) x)
-      \<le> trace_norm (apply_qregister (qregister_inv (qregister_pair C Q)) x)\<close>
-      using trace_norm_sandwich[OF tc, of \<open>tensor_ell2_left (ket c)*\<close>]
-      by simp
-    also have \<open>\<dots> = trace_norm x\<close>
-      apply (rule apply_iso_qregister_trace_norm)
-      apply (auto intro!: iso_qregister_inv_iso simp: )
-      using iso by blast
-    also have \<open>\<dots> = trace_norm x * 1\<close>
-      by simp
-    finally show \<open>trace_norm (sandwich (tensor_ell2_left (ket c)*) *\<^sub>V apply_qregister (qregister_inv (qregister_pair C Q)) x) \<le> \<dots>\<close>
-      by -
-  qed
+  have 1: \<open>cq_operator_at (\<rho> + y) c = cq_operator_at \<rho> c + cq_operator_at y c\<close> for \<rho> y :: \<open>(('a \<times> 'b) ell2, ('a \<times> 'b) ell2) trace_class\<close>
+    by (simp add: sandwich_tc_plus cq_operator_at_def)
+  have 2: \<open>cq_operator_at (r *\<^sub>C \<rho>) c = r *\<^sub>C cq_operator_at \<rho> c\<close> for \<rho> :: \<open>(('a \<times> 'b) ell2, ('a \<times> 'b) ell2) trace_class\<close> and r
+    by (simp add: cq_operator_at_def sandwich_tc_scaleC_right)
+  have 3: \<open>norm (cq_operator_at \<rho> c) \<le> norm \<rho> * 1\<close> for \<rho> :: \<open>(('a \<times> 'b) ell2, ('a \<times> 'b) ell2) trace_class\<close>
+    using norm_sandwich_tc[of \<open>tensor_ell2_left (ket c)*\<close> \<rho>]
+    by (simp add: cq_operator_at_def)
   from 1 2 3
   show ?thesis
     by (rule bounded_clinearI)
 qed
 
-
 lemma cq_operator_reconstruct_inv:
-  fixes C :: \<open>('c, 'a) qregister\<close> and Q :: \<open>('q, 'a) qregister\<close> and \<rho> :: \<open>'c \<Rightarrow> ('q ell2, 'q ell2) trace_class\<close>
-  assumes iso: \<open>iso_qregister (qregister_pair C Q)\<close>
+  fixes \<rho> :: \<open>'c \<Rightarrow> ('q ell2, 'q ell2) trace_class\<close>
   assumes sum_\<rho>: \<open>\<rho> abs_summable_on UNIV\<close>
-  shows \<open>cq_operator_at C Q (cq_operator_reconstruct C Q \<rho>) = \<rho>\<close>
+  shows \<open>cq_operator_at (cq_operator_reconstruct \<rho>) = \<rho>\<close>
 proof (rule ext)
   fix c
-  define CQ CQi where \<open>CQ = qregister_pair C Q\<close> and \<open>CQi = qregister_inv CQ\<close>
-  have dim: \<open>qregister_co_dim CQ = 1\<close>
-    using CQ_def iso iso_qregister_co_dim by blast
-  have *: \<open>cq_operator_at C Q (Abs_trace_class (apply_qregister CQ (selfbutter (ket d) \<otimes>\<^sub>o from_trace_class (\<rho> d)))) c
-    = of_bool (c=d) *\<^sub>C \<rho> d\<close> for d
-  proof (rule from_trace_class_inject[THEN iffD1])
-    have \<open>from_trace_class (cq_operator_at C Q (Abs_trace_class (apply_qregister CQ (selfbutter (ket d) \<otimes>\<^sub>o from_trace_class (\<rho> d)))) c)
-        = sandwich (tensor_ell2_left (ket c)*) (apply_qregister CQi (from_trace_class (Abs_trace_class (apply_qregister CQ (selfbutter (ket d) \<otimes>\<^sub>o from_trace_class (\<rho> d))))))\<close>
-      by (simp add: cq_operator_at.rep_eq CQi_def CQ_def)
-    also have \<open>\<dots> = sandwich (tensor_ell2_left (ket c)*) *\<^sub>V apply_qregister CQi (apply_qregister CQ (selfbutter (ket d) \<otimes>\<^sub>o from_trace_class (\<rho> d)))\<close>
-      apply (subst Abs_trace_class_inverse)
-      by (auto intro!: apply_qregister_trace_class trace_class_tensor iso simp: dim)
-    also have \<open>\<dots> = sandwich (tensor_ell2_left (ket c)*) *\<^sub>V (selfbutter (ket d) \<otimes>\<^sub>o from_trace_class (\<rho> d))\<close>
-      by (auto intro!: simp: CQi_def apply_qregister_inv_inverse iso CQ_def)
-    also have \<open>\<dots> = from_trace_class (of_bool (c = d) *\<^sub>C \<rho> d)\<close>
-      by (simp add: sandwich_tensor_ell2_left)
-    finally show \<open>from_trace_class (cq_operator_at C Q (Abs_trace_class (apply_qregister CQ (selfbutter (ket d) \<otimes>\<^sub>o from_trace_class (\<rho> d)))) c) =
-                  from_trace_class (of_bool (c = d) *\<^sub>C \<rho> d)\<close>
-      by -
-  qed
-  have summable1: \<open>(\<lambda>d. Abs_trace_class (apply_qregister CQ (selfbutter (ket d) \<otimes>\<^sub>o from_trace_class (\<rho> d)))) summable_on UNIV\<close>
-  proof -
-    have tc1: \<open>trace_class (apply_qregister CQ (selfbutter (ket x) \<otimes>\<^sub>o from_trace_class t))\<close> for x t
-      by (auto intro!: apply_qregister_trace_class trace_class_tensor simp: dim)
-    from sum_\<rho> have \<open>(\<lambda>x. trace_norm (selfbutter (ket x) \<otimes>\<^sub>o from_trace_class (\<rho> x))) summable_on UNIV\<close>
-      by (simp add: trace_norm_tensor trace_norm_butterfly flip: norm_trace_class.rep_eq)
-    then have \<open>(\<lambda>x. trace_norm (apply_qregister CQ (selfbutter (ket x) \<otimes>\<^sub>o from_trace_class (\<rho> x)))) summable_on UNIV\<close>
-      apply (subst apply_iso_qregister_trace_norm)
-      by (simp_all add: iso CQ_def)
-    then show ?thesis
-      apply (rule_tac abs_summable_summable)
-      by (simp add: eq_onp_def tc1 norm_trace_class.abs_eq)
-  qed
-  have \<open>cq_operator_at C Q (cq_operator_reconstruct C Q \<rho>) c
-     = cq_operator_at C Q (\<Sum>\<^sub>\<infinity>d. Abs_trace_class (apply_qregister CQ (selfbutter (ket d) \<otimes>\<^sub>o from_trace_class (\<rho> d)))) c\<close>
-    by (simp add: cq_operator_reconstruct_def CQ_def)
-  also have \<open>\<dots> = (\<Sum>\<^sub>\<infinity>d. cq_operator_at C Q (Abs_trace_class (apply_qregister CQ (selfbutter (ket d) \<otimes>\<^sub>o from_trace_class (\<rho> d)))) c)\<close>
-    apply (subst infsum_bounded_linear[where h=\<open>\<lambda>\<rho>. cq_operator_at C Q \<rho> c\<close>])
+  have *: \<open>cq_operator_at (tc_tensor (tc_butterfly (ket d) (ket d)) (\<rho> d)) c = of_bool (c=d) *\<^sub>C \<rho> d\<close> for d
+    apply (rule from_trace_class_inject[THEN iffD1])
+    by (simp add: cq_operator_at_def from_trace_class_sandwich_tc tc_tensor.rep_eq tc_butterfly.rep_eq sandwich_tensor_ell2_left)
+  have summable1: \<open>(\<lambda>c. tc_tensor (tc_butterfly (ket c) (ket c)) (\<rho> c)) summable_on UNIV\<close>
+    by (simp add: abs_summable_summable assms norm_tc_butterfly norm_tc_tensor)
+  have \<open>cq_operator_at (cq_operator_reconstruct \<rho>) c
+     = cq_operator_at (\<Sum>\<^sub>\<infinity>c. tc_tensor (tc_butterfly (ket c) (ket c)) (\<rho> c)) c\<close>
+    by (simp add: cq_operator_reconstruct_def)
+  also have \<open>\<dots> = (\<Sum>\<^sub>\<infinity>d. cq_operator_at (tc_tensor (tc_butterfly (ket d) (ket d)) (\<rho> d)) c)\<close>
+    apply (subst infsum_bounded_linear[where h=\<open>\<lambda>\<rho>. cq_operator_at \<rho> c\<close>])
       apply (simp add: bounded_clinear.bounded_linear cq_operator_at_bounded_clinear) 
      apply (rule summable1)
     by simp
@@ -195,59 +102,37 @@ proof (rule ext)
   also have \<open>\<dots> = \<rho> c\<close>
     apply (subst infsum_single[where i=c])
     by auto
-  finally show \<open>cq_operator_at C Q (cq_operator_reconstruct C Q \<rho>) c = \<rho> c\<close>
+  finally show \<open>cq_operator_at (cq_operator_reconstruct \<rho>) c = \<rho> c\<close>
     by -
 qed
 
 lemma cq_operator_reconstruct:
-  assumes iso: \<open>iso_qregister (qregister_pair C Q)\<close>
-  assumes cq: \<open>classical_on C \<rho>\<close>
-  shows \<open>cq_operator_reconstruct C Q (cq_operator_at C Q \<rho>) = \<rho>\<close>
+  fixes \<rho> :: \<open>(('c\<times>'q) ell2, ('c\<times>'q) ell2) trace_class\<close>
+  assumes cq: \<open>classical_fst \<rho>\<close>
+  shows \<open>cq_operator_reconstruct (cq_operator_at \<rho>) = \<rho>\<close>
 proof -
-  define CQ CQi where \<open>CQ = qregister_pair C Q\<close> and \<open>CQi = qregister_inv CQ\<close>
-
-  from iso
-  have [simp]: \<open>qregister_co_dim CQ = 1\<close>
-    using CQ_def iso_qregister_co_dim by blast
-
-  have [simp]: \<open>qregister_co_dim CQi = 1\<close>
-    by (simp add: CQ_def CQi_def assms(1) iso_qregister_co_dim iso_qregister_inv_iso)
-
-  have \<open>cq_operator_reconstruct C Q (cq_operator_at C Q \<rho>)
-        = (\<Sum>\<^sub>\<infinity>c. Abs_trace_class (apply_qregister CQ (selfbutter (ket c) \<otimes>\<^sub>o sandwich (tensor_ell2_left (ket c)*) *\<^sub>V apply_qregister CQi (from_trace_class \<rho>))))\<close>
-    by (simp add: cq_operator_reconstruct_def cq_operator_at.rep_eq CQ_def CQi_def)
-  also have \<open>\<dots> = (\<Sum>\<^sub>\<infinity>c. sandwich_tc (apply_qregister C (selfbutter (ket c))) \<rho>)\<close>
+  define f :: \<open>('c \<times> 'q) ell2 \<Rightarrow>\<^sub>C\<^sub>L ('c \<times> 'q) ell2 \<Rightarrow> 'c ell2 \<Rightarrow>\<^sub>C\<^sub>L 'c ell2\<close>
+    where \<open>f = inv (\<lambda>E. E \<otimes>\<^sub>o id_cblinfun)\<close>
+  have [simp]: \<open>f (E \<otimes>\<^sub>o id_cblinfun) = E\<close> for E :: \<open>'c ell2 \<Rightarrow>\<^sub>C\<^sub>L 'c ell2\<close>
+    unfolding f_def
+    apply (subst inv_f_f)
+    by (auto intro!: inj_tensor_left)
+  have \<open>cq_operator_reconstruct (cq_operator_at \<rho>)
+        = (\<Sum>\<^sub>\<infinity>c. (tc_tensor (tc_butterfly (ket c) (ket c)) (sandwich_tc (tensor_ell2_left (ket c)*) \<rho>)))\<close>
+    by (simp add: cq_operator_reconstruct_def cq_operator_at_def)
+  also have \<open>\<dots> = (\<Sum>\<^sub>\<infinity>c. sandwich_tc (selfbutter (ket c) \<otimes>\<^sub>o id_cblinfun) \<rho>)\<close>
     (is \<open>(\<Sum>\<^sub>\<infinity>c. ?lhs c) = (\<Sum>\<^sub>\<infinity>c. ?rhs c)\<close>)
   proof (rule infsum_cong)
     fix c
-    have \<open>?lhs c
-        = apply_qregister_tc CQ
-                  (Abs_trace_class  (selfbutter (ket c) \<otimes>\<^sub>o sandwich (tensor_ell2_left (ket c)*) *\<^sub>V apply_qregister CQi (from_trace_class \<rho>)))\<close>
-      apply (subst apply_qregister_tc.abs_eq)
-       apply (simp add: apply_qregister_trace_class eq_onp_def trace_class_sandwich trace_class_tensor)
-      by simp
-    also have \<open>\<dots> = apply_qregister_tc CQ (tc_tensor (tc_butterfly (ket c) (ket c))
-       (sandwich_tc (tensor_ell2_left (ket c)*) (Abs_trace_class (apply_qregister CQi (from_trace_class \<rho>)))))\<close>
-      by (simp add: eq_onp_def apply_qregister_trace_class trace_class_sandwich
-          flip: tc_butterfly.abs_eq tc_tensor.abs_eq sandwich_tc_Abs_trace_class)
-    also have \<open>\<dots> = apply_qregister_tc CQ (tc_tensor (tc_butterfly (ket c) (ket c))
-       (sandwich_tc (tensor_ell2_left (ket c)*) (apply_qregister_tc CQi (Abs_trace_class (from_trace_class \<rho>)))))\<close>
-      apply (subst apply_qregister_tc.abs_eq)
-      by (simp_all add: eq_onp_def)
-    also have \<open>\<dots> = apply_qregister_tc CQ
-     (tc_tensor (tc_butterfly (ket c) (ket c))
-       (sandwich_tc (tensor_ell2_left (ket c)*) (apply_qregister_tc CQi \<rho>)))\<close>
-      by (simp add: from_trace_class_inverse)
-    also have \<open>\<dots> = apply_qregister_tc CQ (sandwich_tc (selfbutter (ket c) \<otimes>\<^sub>o id_cblinfun) (apply_qregister_tc CQi \<rho>))\<close>
+    show \<open>?lhs c = ?rhs c\<close>
     proof -
       have *: \<open>sandwich_tc (selfbutter (ket c) \<otimes>\<^sub>o id_cblinfun) (tc_tensor x (tc_butterfly a b)) =
        tc_tensor (tc_butterfly (ket c) (ket c)) (sandwich_tc (tensor_ell2_left (ket c)*) (tc_tensor x (tc_butterfly a b)))\<close>
-        for x :: \<open>('a ell2, 'a ell2) trace_class\<close> and a b :: \<open>'e ell2\<close>
+        for x :: \<open>('c ell2, 'c ell2) trace_class\<close> and a b :: \<open>'e ell2\<close>
         apply (rule from_trace_class_inject[THEN iffD1])
         apply (simp add: from_trace_class_sandwich_tc tc_tensor.rep_eq tc_butterfly.rep_eq sandwich_tensor_ell2_left)
         by (simp add: sandwich_apply tensor_op_adjoint comp_tensor_op butterfly_comp_cblinfun cinner_adj_left tensor_op_cbilinear.scaleC_left tensor_op_cbilinear.scaleC_right)
-      have \<open>sandwich_tc (selfbutter (ket c) \<otimes>\<^sub>o id_cblinfun) = (\<lambda>\<rho>. tc_tensor (tc_butterfly (ket c) (ket c))
-       (sandwich_tc (tensor_ell2_left (ket c)*) \<rho>))\<close>
+      have \<open>sandwich_tc (selfbutter (ket c) \<otimes>\<^sub>o id_cblinfun) = (\<lambda>\<rho>. tc_tensor (tc_butterfly (ket c) (ket c)) (sandwich_tc (tensor_ell2_left (ket c)*) \<rho>))\<close>
         apply (rule eq_from_separatingI2)
            apply (rule separating_set_bounded_clinear_tc_tensor_nested)
             apply (rule separating_set_UNIV)
@@ -258,24 +143,19 @@ proof -
       then show ?thesis
         by metis
     qed
-    also have \<open>\<dots> = sandwich_tc (apply_qregister CQ (selfbutter (ket c) \<otimes>\<^sub>o id_cblinfun)) (apply_qregister_tc CQ (apply_qregister_tc CQi \<rho>))\<close>
-      by (rule apply_qregister_tc_sandwich)
-    also have \<open>\<dots> = sandwich_tc (apply_qregister CQ (selfbutter (ket c) \<otimes>\<^sub>o id_cblinfun)) \<rho>\<close>
-      using \<open>qregister_co_dim CQ = 1\<close> \<open>qregister_co_dim CQi = 1\<close> 
-      by (smt (verit, ccfv_SIG) CQ_def CQi_def apply_qregister_inv_inverse apply_qregister_tc.rep_eq from_trace_class_inverse iso iso_qregister_inv_iso one_neq_zero)
-    also have \<open>\<dots> = sandwich_tc (apply_qregister C (selfbutter (ket c))) \<rho>\<close>
-      by (metis CQ_def apply_qregister_extend_pair_right assms(1) iso_qregister_def')
-    finally show \<open>?lhs c = ?rhs c\<close>
-      by -
   qed
-  also have \<open>\<dots> = (\<Sum>\<^sub>\<infinity>E\<in>range (\<lambda>x::'a. (apply_qregister C (selfbutter (ket x)), ket x)). sandwich_tc (fst E) \<rho>)\<close>
+  also have \<open>\<dots> = (\<Sum>\<^sub>\<infinity>E\<in>range (\<lambda>x::'c. ((selfbutter (ket x) \<otimes>\<^sub>o id_cblinfun), ket x)). sandwich_tc (fst E) \<rho>)\<close>
     apply (subst infsum_reindex)
-    by (simp_all add: inj_def o_def) 
-  also have \<open>\<dots> = kraus_family_map (apply_qregister_kraus_map C (complete_measurement (range ket))) \<rho>\<close>
-    apply (transfer' fixing: \<rho> C)
-    apply (simp add: image_image)
-    apply transfer' (* Need to do this because the first transfer transferred a "ket x" that we didn't want transferred. *)
-    by simp
+    by (simp_all add: inj_def o_def)
+  also have \<open>\<dots> = (\<Sum>\<^sub>\<infinity>((E, x), F, y)\<in>range (\<lambda>x. (selfbutter (ket x), ket x)) \<times> {(id_cblinfun, ())}. sandwich_tc (E \<otimes>\<^sub>o F) \<rho>)\<close>
+    apply (subst infsum_reindex_bij_betw[where A=\<open>range (\<lambda>x. (selfbutter (ket x), ket x)) \<times> {(id_cblinfun, ())}\<close>
+          and g=\<open>\<lambda>((E,x),(F,y)). (E \<otimes>\<^sub>o F, x)\<close>, symmetric])
+     apply (rule bij_betw_byWitness[where f'=\<open>\<lambda>(Eid,x). ((f Eid,x),(id_cblinfun,()))\<close>])
+        apply auto[4]
+    by (simp add: case_prod_unfold)
+  also have \<open>\<dots> = kraus_family_map (kraus_family_tensor (complete_measurement (range ket)) kraus_family_id) \<rho>\<close>
+    apply (simp only: kraus_family_map_tensor_sum kraus_family_id_def kraus_family_of_op.rep_eq complete_measurement.rep_eq)
+    by (simp add: image_image)
   also have \<open>\<dots> = \<rho>\<close>
     by (metis cq classical_on_def)
   finally show ?thesis
